Steel.Repr.ST: binders flattening

experiment/Experiment.Steel.Repr.ST.fst
@@ -5,6 +5,41 @@ module T = FStar.Tactics
 open FStar.Calc
 
 
+(***** [equiv] *)
+
+#push-options "--ifuel 0"
+
+let equiv_Tframe #a #pre #post frame f f' eq_f
+  = _ by T.(//unfold one level of tree_ens / tree_req
+            norm [delta_only [`%equiv; `%tree_req; `%tree_ens]; zeta];
+            norm [iota];
+            smt ())
+
+let equiv_Tbind #a #b #pre #itm #post f f' g g' eq_f eq_g
+  = let eq_g = FStar.Classical.forall_intro_squash_gtot eq_g in
+    _ by T.(norm [delta_only [`%equiv; `%tree_req; `%tree_ens]; zeta];
+            norm [iota];
+            smt ())
+
+let equiv_TbindP #a #b #pre #post wp f g g' eq_g
+  =
+    FStar.Classical.forall_intro_squash_gtot eq_g;
+    FStar.Monotonic.Pure.elim_pure_wp_monotonicity wp;
+    assert (equiv (TbindP a b pre post wp f g) (TbindP a b pre post wp f g'))
+      by T.(norm [delta_only [`%equiv; `%tree_req; `%tree_ens]; zeta];
+            norm [iota];
+            smt ())
+
+let equiv_Tbind_assoc_Tbind #a #b #c #pre #itm0 #itm1 #post f g h
+  : squash (equiv (bind (bind f g) h) (bind f (fun x -> bind (g x) h)))
+  = _ by T.(norm [delta_only [`%equiv; `%tree_req; `%tree_ens; `%bind]; zeta];
+            norm [iota];
+            smt ())
+
+#pop-options
+
+(**) let __begin_shape = ()
+
 (**** soundness of M --> ST *)
 
 (***** Spec *)
@@ -267,4 +302,111 @@ let rec repr_ST_of_M_shape
             let M.SbindP _ _ s_g = s in
             introduce forall (x : a) . prog_has_shape (repr_ST_of_M (g x) (cg x)) (shape_ST_of_M s_g)
               with repr_ST_of_M_shape (g x) (cg x) s_g
+#pop-options
+
+
+(*** Binders flattening *)
+
+#push-options "--fuel 2 --ifuel 1"
+let rec flatten_equiv
+      #a #pre #post (t : prog_tree u#a u#b a pre post)
+  : Lemma (ensures equiv (flatten_prog t) t) (decreases %[t; 1])
+  = flatten_equiv_aux t flatten_prog_k_id
+      (fun _ _ _ -> ()) (fun _ _ _ _ _ -> ())
+
+and flatten_equiv_aux
+      #a  #pre #post (t : prog_tree u#a u#b a pre post)
+      #a1 #post1 (k : ((#pre' : pre_t) -> (t' : prog_tree a pre' post) -> prog_tree a1 pre' post1))
+      (k_equiv : (pre' : pre_t) -> (t'0 : prog_tree a pre' post) -> (t'1 : prog_tree a pre' post) ->
+                     Lemma (requires equiv t'0 t'1) (ensures equiv (k t'0) (k t'1)))
+      (k_bind  : ((a0 : Type u#a) -> (pre' : pre_t) -> (itm : post_t a0) ->
+                      (f : prog_tree a0 pre' itm) -> (g : ((x : a0) -> (prog_tree a (itm x) post))) ->
+                     Lemma (equiv (k (Tbind a0 a pre' itm post f g))
+                                  (Tbind a0 a1 pre' itm post1 f (fun x -> k (g x))))))
+  : Lemma (ensures equiv (flatten_prog_aux t k) (k t)) (decreases %[t; 0])
+  = match t with
+  | Tequiv _ _ _ | Tspec _ _ _ _ _ | Tret _ _ _ -> ()
+  | Tframe a pre post frame f ->
+             equiv_Tframe frame (flatten_prog f) f (flatten_equiv f);
+             k_equiv _ (Tframe _ _ _ frame (flatten_prog f)) t
+  | Tbind  a b pre itm post f g ->
+             let t = Tbind a b pre itm post f g in
+             let g1 (x : a) = flatten_prog_aux (g x) k in
+             let g2 (x : a) = k (g x) in
+             let k1 (#pre' : pre_t) (f' : prog_tree a pre' itm) =
+               Tbind a a1 pre' itm post1 f' g1
+             in
+             assert (flatten_prog_aux t k == flatten_prog_aux f k1)
+               by T.(trefl ());
+             flatten_equiv_aux f k1
+               (fun _ t'0 t'1 -> equiv_Tbind t'0 t'1 g1 g1 () (fun _ -> ()))
+               (fun a0 pre' itm f' g' -> equiv_Tbind_assoc_Tbind f' g' g1);
+             equiv_Tbind f f g1 g2
+               () (fun (x : a) -> flatten_equiv_aux (g x) k k_equiv k_bind);
+             assert (equiv (flatten_prog_aux t k) (Tbind a a1 pre itm post1 f g2));
+             k_bind _ _ _ f g
+  | TbindP a b pre post wp f g ->
+             let t = TbindP a b pre post wp f g in
+             let g1 (x : a) = flatten_prog (g x) in
+             assert (flatten_prog_aux t k == k (TbindP _ _ _ _ wp f g1))
+               by T.(trefl ());
+             equiv_TbindP wp f g1 g
+               (fun x -> flatten_equiv (g x));
+             k_equiv _ (TbindP _ _ _ _ wp f g1) t
+
+let rec flatten_prog_shape
+      #a #pre #post (t : prog_tree u#a u#b a pre post)
+      (#post_n : nat) (s : shape_tree (L.length pre) post_n)
+   : Lemma (requires prog_has_shape t s)
+           (ensures  prog_has_shape (flatten_prog t) (flatten_shape s))
+           (decreases %[t; 1])
+   = flatten_prog_shape_aux t s flatten_prog_k_id post_n flatten_shape_k_id (fun _ _ _ -> ())
+
+and flatten_prog_shape_aux
+      #a #pre #post (t : prog_tree u#a u#b a pre post)
+      (#post_n : nat) (s : shape_tree (L.length pre) post_n)
+      #a1 #post1 (k_t : ((#pre' : pre_t) -> (t' : prog_tree a pre' post) -> prog_tree u#a u#b a1 pre' post1))
+      (post1_n : nat {post_has_len post1 post1_n})
+      (k_s : ((#pre'_n : nat) -> (s' : shape_tree pre'_n post_n) -> shape_tree pre'_n post1_n))
+      (k_hyp : (pre' : pre_t) -> (t' : prog_tree a pre' post) -> (s' : shape_tree (L.length pre') post_n) ->
+                   Lemma (requires prog_has_shape t' s') (ensures prog_has_shape (k_t t') (k_s s')))
+   : Lemma (requires prog_has_shape t s)
+           (ensures  prog_has_shape (flatten_prog_aux t k_t) (flatten_shape_aux s k_s))
+           (decreases %[t; 0])
+   = match t with
+  | Tequiv _ _ _ | Tspec _ _ _ _ _ | Tret _ _ _ ->
+           k_hyp _ t s
+  | Tframe a pre post frame f ->
+           let Sframe _ _ frame_n s_f = s in
+           flatten_prog_shape f s_f;
+           k_hyp _ (Tframe _ _ _ frame (flatten_prog f))
+                       (Sframe _ _ frame_n (flatten_shape s_f))
+  | Tbind  a b pre itm post f g ->
+           let t = Tbind a b pre itm post f g in
+           let Sbind pre_n itm_n post_n s_f s_g = s in
+           let s = Sbind pre_n itm_n post_n s_f s_g in
+           let g1 (x : a) = flatten_prog_aux (g x) k_t in
+           let k_t1 (#pre' : pre_t) (f' : prog_tree a pre' itm) =
+             Tbind a a1 pre' itm post1 f' g1
+           in let k_s1 (#pre'_n : nat) (s_f' : shape_tree pre'_n itm_n) =
+             Sbind _ itm_n _ s_f' (flatten_shape_aux s_g k_s)
+           in
+           assert (flatten_prog_aux t k_t == flatten_prog_aux f k_t1)
+             by T.(trefl ());
+           assert (flatten_shape_aux s k_s == flatten_shape_aux s_f k_s1)
+             by T.(trefl ());
+           flatten_prog_shape_aux f s_f k_t1 post1_n k_s1
+             (fun pre' t' s' ->
+               introduce forall (x : a) . prog_has_shape (g1 x) (flatten_shape_aux s_g k_s)
+                 with flatten_prog_shape_aux (g x) s_g k_t post1_n k_s k_hyp)
+  | TbindP a b pre post wp f g ->
+           let t = TbindP a b pre post wp f g in
+           let SbindP _ _ s_g = s in
+           let g1 (x : a) = flatten_prog (g x) in
+           assert (flatten_prog_aux t k_t == k_t (TbindP _ _ _ _ wp f g1))
+             by T.(trefl ());
+           introduce forall (x : a) . prog_has_shape (g1 x) (flatten_shape s_g)
+             with flatten_prog_shape (g x) s_g;
+           k_hyp _ (TbindP _ _ _ _ wp f g1) (SbindP _ _ (flatten_shape s_g))
+
 #pop-options
